formal/Weft.lean
@@ -12,6 +12,7 @@ import Weft.Properties.CoreEffectSoundness
 import Weft.Properties.CorePipelineCorrectness
 import Weft.Properties.CoreSemanticSoundness
 import Weft.Properties.CoreSubtypeSoundness
+import Weft.Properties.CoreTypecheckCorrectness
 import Weft.Properties.CompilerCorrectness
 import Weft.Properties.EffectDiscipline
 import Weft.Properties.TypeSafetyCore
